\begin{equation}
\begin{aligned}
\mathbf{M}^f_{\Sigma^{-1}} &=
    \frac{1}{2^d}
    \left(\sum_{i=1}^{2^d}
        \mathbf{Q}_i^{\top} \mathbf{N}_i^{-\top} \sqrt{v_{\text{cell}}}
            ~ \Sigma^{-1}
        \sqrt{v_{\text{cell}}}  ~ \mathbf{N}_i^{-1} \mathbf{Q}_i
    \right)
\\
& =
    \sum_{i=1}^{2^d}
    \mathbf{P}_i^\top \Sigma^{-1} \mathbf{P}_i , \qquad \text{where}\\
\mathbf{P}_i & = \sqrt{ \frac{1}{2^d} \mathbf{I}^d \otimes \text{diag} \left( \mathbf{v} \right)} \mathbf{N}_i^{-1} \mathbf{Q}_i
\end{aligned}
\end{equation}
