\begin{equation}
\begin{aligned}
n_c &= n_{c_x} \times n_{c_y} \times n_{c_z}                    & \text{cells}\\
n_n &= (n_{c_x} + 1) \times (n_{c_y} + 1) \times (n_{c_z} +1)   & \text{nodes}\\
n_{f_x} &= (n_{c_x} + 1) \times n_{c_y} \times n_{c_z}          & \text{x-faces}\\
n_{f_y} &= n_{c_x} \times (n_{c_y} + 1) \times n_{c_z}          & \text{y-faces}\\
n_{f_z} &= n_{c_x} \times n_{c_y} \times (n_{c_z} + 1)          & \text{z-faces}\\
n_{e_x} &= n_{c_x} \times (n_{c_y} + 1) \times (n_{c_z} + 1)    & \text{x-edges}\\
n_{e_y} &= (n_{c_x} + 1) \times n_{c_y} \times (n_{c_z} + 1)    & \text{y-edges}\\
n_{e_z} &= (n_{c_x} + 1) \times (n_{c_y} + 1) \times n_{c_z}    & \text{z-edges}\\
\end{aligned}
\end{equation}
